retrieve wip

theories/lang.v
@@ -188,9 +188,7 @@ Definition update_access_global_batch st (v:VMID) (ps : list PID) (pm: access): 
    get_mem st, get_transactions st).
 
 Definition update_memory_global_batch (st : state) (l : list (Addr * Word)) : state :=
-  (get_reg_files st, get_mail_boxes st, get_page_tables st, get_current_vm st,
-   (foldr (λ p acc, match p with | (a, w) => <[a:=w]>acc end) (snd (fst st)) l),
-           get_transactions st).
+  (get_reg_files st, get_mail_boxes st, get_page_tables st, get_current_vm st, (list_to_map l) ∪ (get_mem st), get_transactions st).
 
 Definition update_ownership_batch st (ps : list PID) (pm: ownership): state :=
   update_ownership_global_batch st (get_current_vm st) ps pm.
@@ -436,35 +434,34 @@ Definition empty_rx_global (st : state) (v : VMID) : option state :=
 Definition empty_rx (st : state) : option state :=
   empty_rx_global st (get_current_vm st).
 
-Definition copy_from_addr_to_addr_unsafe (st : state) (src dst : Addr) : option state :=
-  w <- get_memory_unsafe st src ;;;
-  Some (update_memory_unsafe st dst w).
+Definition write_mem_segment_unsafe (st : state) (dst : Addr) (segment : list Word) : state :=
+  update_memory_global_batch st (zip (finz.seq dst (Z.to_nat page_size)) segment).
 
-Definition copy_page_unsafe (st : state) (src dst : PID) : option state :=
-  foldr (fun x s =>
-           match x with
-           | (a, b) =>
-             (@bind option _ _ _ state state s (fun y => copy_from_addr_to_addr_unsafe y a b))
-           end)
-        (Some st)
-        (zip (finz.seq (of_pid src)  (Z.to_nat page_size))
-                   (finz.seq (of_pid dst)  (Z.to_nat page_size))).
+Definition read_mem_segment_unsafe (st : state) (src : Addr) (l : Word) : list Word :=
+  foldr (fun x s => match get_memory_unsafe st x with | Some x' => x' :: s | None => s end) [] (finz.seq src (Z.to_nat (finz.to_z l))).
 
-Program Definition transfer_msg_unsafe (st : state) (l : Word) (v : VMID) (r : VMID) : hvc_result state :=
-  if (l <? page_size)%Z then
-    match get_vm_mail_box st v with
-    | (txPid, _) =>
-      match get_vm_mail_box st r with
-      | (tx, (rxPid, _)) =>
-        st' <- lift_option (copy_page_unsafe st txPid rxPid) ;;;
-        unit (get_reg_files st,
-              vinsert r (tx, (rxPid, Some(l, v))) (get_mail_boxes st),
-              get_page_tables st,
-              get_current_vm st,
-              get_mem st', get_transactions st)
-      end
-    end
-  else throw InvParam.
+Definition copy_from_addr_to_addr_unsafe (st : state) (src dst : Addr) (l : Word) : state :=
+  write_mem_segment_unsafe st dst (read_mem_segment_unsafe st src l).
+
+Definition copy_page_segment_unsafe (st : state) (src dst : PID) (l : Word) : state :=
+  copy_from_addr_to_addr_unsafe st (of_pid src) (of_pid dst) l.
+
+Definition fill_rx_unsafe (st : state) (l : Word) (v r : VMID) (tx rx : PID) : state :=
+  (get_reg_files st, vinsert r (tx, (rx, Some(l, v))) (get_mail_boxes st), get_page_tables st, get_current_vm st, get_mem st, get_transactions st).
+
+Definition fill_rx (st : state) (l : Word) (v r : VMID) : hvc_result state :=
+  match get_vm_mail_box st r with
+  | (tx, (rx, None)) =>
+    unit (fill_rx_unsafe st l v r tx rx)
+  | _ => throw Busy
+  end.
+
+Definition transfer_msg_unsafe (st : state) (l : Word) (v : VMID) (r : VMID) : hvc_result state :=
+  if (page_size <? l)%Z
+  then throw InvParam
+  else
+    let st' := copy_page_segment_unsafe st (get_tx_pid_global st v) (get_rx_pid_global st r) l
+    in fill_rx st' l v r.
 
 Definition transfer_msg (st : state) (l : Word) (r : VMID) : hvc_result state :=
   transfer_msg_unsafe st l (get_current_vm st) r.
@@ -496,9 +493,6 @@ Definition transaction_to_transaction_descriptor (t : transaction) (h : handle) 
   | (vs, f, _, vr, ls, _) => (vs, Some h, f, vr, ls)
   end.
 
-Definition write_mem_segment_page_unsafe (st : state) (dst : PID) (segment : list Word) : state :=
-  update_memory_global_batch st (zip (finz.seq (of_pid dst) (Z.to_nat page_size)) segment).
-
 Definition transaction_to_list_words (t : transaction) (h : handle) : option (list Word) :=
   match transaction_to_transaction_descriptor t h with
   | (vs, Some h, f, vr, ls) =>
@@ -517,7 +511,7 @@ Definition transaction_to_list_words (t : transaction) (h : handle) : option (li
 
 Definition transaction_write_rx (st : state) (t : transaction) (h : handle) : option state :=
   match transaction_to_list_words t h with
-  | Some ls => Some (write_mem_segment_page_unsafe st (get_rx_pid_global st (get_current_vm st)) ls)
+  | Some ls => Some (write_mem_segment_unsafe st (get_rx_pid_global st (get_current_vm st)) ls)
   | None => None
   end.
 
@@ -534,9 +528,11 @@ Definition parse_memory_region_descriptor (st : state) (b:Addr) : option memory_
 
 Definition parse_transaction_descriptor_retrieve (st : state) (b : Addr) : option transaction_descriptor :=
   vs <- get_memory_with_offset st b 0 ;;;
+  wf <- get_memory_with_offset st b 1 ;;;
   wh <- get_memory_with_offset st b 2 ;;;
   vs' <- decode_vmid vs ;;;
-  unit (vs', Some wh, W0, (get_current_vm st), []).
+  unit (vs', Some wh, wf, (get_current_vm st), []).
+
 (* TODO: Prop version, reflection *)
 
 Definition parse_transaction_descriptor (st : state) (b: Addr) : option transaction_descriptor :=
@@ -549,6 +545,7 @@ Definition parse_transaction_descriptor (st : state) (b: Addr) : option transact
   unit (vs', (if (finz.to_z wh =? 0)%Z then None else Some wh), wf, md.1, md.2).
 
 (*TODO: validate length*)
+
 Definition validate_transaction_descriptor (st : state) (wl : Word) (ty : transaction_type)
            (t : transaction_descriptor) : hvc_result () :=
   match t with
@@ -573,7 +570,6 @@ Definition validate_transaction_descriptor (st : state) (wl : Word) (ty : transa
            ) InvParam ;;;
     unit tt
   end.
-
 
 Definition insert_transaction (st : state) (h : handle) (t : transaction) : state :=
   (get_reg_files st, get_mail_boxes st, get_page_tables st, get_current_vm st, get_mem st,
@@ -721,7 +717,7 @@ Definition retrieve (s : state) : exec_mode * state :=
          let ty := get_transaction_type trn in
          (* add receiver(caller) into the list of the transaction *)
          s' <- toggle_transaction_retrieve s handle trn ;;;
-         s'' <- lift_option_with_err (transaction_write_rx s trn handle) InvParam ;;;
+         s'' <- transfer_msg s' len (get_current_vm s') ;;;
          (* for all pages of the trancation ... (change the page table of the caller according to the type)*)
          match ty with
          | Sharing =>
